dafny/abstract-interpreter/BoundedInts.dfy
@@ -8,13 +8,13 @@ module BoundedInts {
   const TWO_TO_THE_4:   int := 16
   const TWO_TO_THE_5:   int := 32
   const TWO_TO_THE_8:   int := 0x100
-  const TWO_TO_THE_16:  int := 0x10000
-  const TWO_TO_THE_24:  int := 0x1000000
-  const TWO_TO_THE_32:  int := 0x1_00000000
-  const TWO_TO_THE_40:  int := 0x100_00000000
-  const TWO_TO_THE_48:  int := 0x10000_00000000
-  const TWO_TO_THE_56:  int := 0x1000000_00000000
-  const TWO_TO_THE_64:  int := 0x1_00000000_00000000
+  const TWO_TO_THE_16:  int := 0x1_0000
+  const TWO_TO_THE_24:  int := 0x100_0000
+  const TWO_TO_THE_32:  int := 0x1_0000_0000
+  const TWO_TO_THE_40:  int := 0x100_0000_0000
+  const TWO_TO_THE_48:  int := 0x1_0000_0000_0000
+  const TWO_TO_THE_56:  int := 0x100_0000_0000_0000
+  const TWO_TO_THE_64:  int := 0x1_0000_0000_0000_0000
 
   const S64_MIN : int64 := -0x8000_0000_0000_0000
   const S64_MAX : int64 := (0x8000_0000_0000_0000 - 1) as int64
@@ -27,15 +27,15 @@ module BoundedInts {
   const U32_MAX : uint32 := 0x8000_0000 - 1
 
 
-  newtype int8  = x: int  | -0x80 <= x < 0x80
-  newtype int16 = x: int  | -0x8000 <= x < 0x8000
-  newtype int32 = x: int  | -0x8000_0000 <= x < 0x8000_0000
-  newtype int64 = x: int  | -0x8000_0000_0000_0000 <= x < 0x8000_0000_0000_0000
+  newtype int8  = x: int | -0x80 <= x < 0x80
+  newtype int16 = x: int | -0x8000 <= x < 0x8000
+  newtype int32 = x: int | -0x8000_0000 <= x < 0x8000_0000
+  newtype int64 = x: int | -0x8000_0000_0000_0000 <= x < 0x8000_0000_0000_0000
 
-  newtype uint8 = x:int | 0 <= x < 0x100
-  newtype uint16 = x:int | 0 <= x < 0x1_0000
-  newtype uint32 = x:int | 0 <= x < 0x1_0000_0000
-  newtype uint64 = x:int | 0 <= x < 0x1_00000000_00000000
+  newtype uint8  = x: int | 0 <= x < 0x100
+  newtype uint16 = x: int | 0 <= x < 0x1_0000
+  newtype uint32 = x: int | 0 <= x < 0x1_0000_0000
+  newtype uint64 = x: int | 0 <= x < 0x1_0000_0000_0000_0000
 
 
   type byte = uint8
